Carrier/KozenExample.thy
@@ -4,14 +4,91 @@ begin
 
 (* Kozen and Angus's example *)
 
+lemma zip_elim_var: "x\<cdot>y = y \<Longrightarrow> qes (x#xs) \<cdot> seq (y#ys) = qes xs \<cdot> seq (y#ys)"
+  by (metis (lifting) seq_cons skd.mult_assoc zip_left)
+
+lemma test_under_one: "p \<in> carrier tests \<Longrightarrow> p \<sqsubseteq> \<one>"
+  by (metis skt.test_under_one)
+
+lemma test_double_compl: "p \<in> carrier tests \<Longrightarrow> p = !(!p)"
+  by (metis kat_comp_simp not_closed skt.test_double_compl)
+
+lemma de_morgan1: "\<lbrakk>p \<in> carrier tests; q \<in> carrier tests\<rbrakk> \<Longrightarrow> !p \<cdot> !q = !(p + q)"
+  by (smt kat_comp_simp skt.de_morgan1 test_plus_closed)
+
+lemma test_meet_def: "\<lbrakk>p \<in> carrier tests; q \<in> carrier tests\<rbrakk> \<Longrightarrow> p \<cdot> q = !(!p + !q)"
+  by (metis (lifting) de_morgan1 not_closed test_double_compl)
+
+lemma de_morgan2: "\<lbrakk>p \<in> carrier tests; q \<in> carrier tests\<rbrakk> \<Longrightarrow> !p + !q = !(p \<cdot> q)"
+  by (smt not_closed test_double_compl test_meet_def test_plus_closed)
+
+lemma test_compl_anti: "\<lbrakk>p \<in> carrier tests; q \<in> carrier tests\<rbrakk> \<Longrightarrow> p \<sqsubseteq> q \<longleftrightarrow> !q \<sqsubseteq> !p"
+  by (metis kat_comp_simp skt.test_compl_anti)
+
+lemma test_join_def: "\<lbrakk>p \<in> carrier tests; q \<in> carrier tests\<rbrakk> \<Longrightarrow> p + q = !(!p \<cdot> !q)"
+  by (metis (lifting) de_morgan2 not_closed test_double_compl)
+
+lemma ba_3: "\<lbrakk>p \<in> carrier tests; q \<in> carrier tests\<rbrakk> \<Longrightarrow> p = (p \<cdot> q) + (p \<cdot> !q)"
+  by (metis Ranked_Alphabet.mult_oner complement_one skd.distl)
+
+lemma ba_5: "\<lbrakk>p \<in> carrier tests; q \<in> carrier tests\<rbrakk> \<Longrightarrow> (p + q) \<cdot> !p = q \<cdot> !p"
+  by (metis (lifting) complement_zero skd.add_zerol skd.distr)
+
+lemma compl_1: "\<lbrakk>p \<in> carrier tests; q \<in> carrier tests\<rbrakk> \<Longrightarrow> !p = !(p + q) + !(p + !q)"
+  by (metis (lifting) ba_3 de_morgan1 not_closed)
+
+lemma ba_1: "\<lbrakk>p \<in> carrier tests; q \<in> carrier tests; r \<in> carrier tests\<rbrakk> \<Longrightarrow> p + q + !q = r + !r"
+  by (metis Ranked_Alphabet.mult_oner complement_one ska.star_unfoldl_eq skd.add_assoc skd.add_comm skt.test_star)
+
+lemma ba_2: "\<lbrakk>p \<in> carrier tests; q \<in> carrier tests\<rbrakk> \<Longrightarrow> p + p = p + !(q + !q)"
+  by (metis complement_one kat_comp_simp skd.add_idem skd.add_zeror skt.test_not_one test_one_closed)
+
+lemma ba_4: "\<lbrakk>p \<in> carrier tests; q \<in> carrier tests\<rbrakk> \<Longrightarrow> p = (p + !q) \<cdot> (p + q)"
+  by (metis complement_zero not_closed skd.add_zeror skt.test_dist2 skt.test_mult_comm)
+
+lemma shunting:
+  assumes pc: "p \<in> carrier tests" and qc: "q \<in> carrier tests" and rc: "r \<in> carrier tests"
+  shows "p \<cdot> q \<sqsubseteq> r \<longleftrightarrow> q \<sqsubseteq> !p + r"
+  by (metis kat_comp_simp pc qc rc skt.shunting)
+
+fun break' :: "'a list \<Rightarrow> nat \<Rightarrow> 'a list \<Rightarrow> ('a list \<times> 'a list)" where
+  "break' ac 0 xs = (rev ac, xs)"
+| "break' ac (Suc n) [] = (rev ac, [])"
+| "break' ac (Suc n) (x#xs) = break' (x#ac) n xs"
+
+abbreviation break :: "nat \<Rightarrow> 'a list \<Rightarrow> ('a list \<times> 'a list)" where
+  "break \<equiv> break' []"
+
+inductive comms :: "'a::ranked_alphabet skat \<Rightarrow> 'a skat list \<Rightarrow> bool" where
+  comms_nil: "comms x []"
+| comms_cons: "\<lbrakk>x\<cdot>y = y\<cdot>x; comms x ys\<rbrakk> \<Longrightarrow> comms x (y#ys)"
+
+lemma comm_step:
+  assumes "\<exists>i. nth ys i = x \<and> comms x (fst (break i ys)) \<and> seq xs = seq (fst (break i ys) @ tl (snd (break i ys)))"
+  shows "seq (x#xs) = seq ys"
+  sorry
+
 (* Defining the alphabet *)
 
 definition biconditional ::
   "'a::ranked_alphabet skat \<Rightarrow> 'a skat \<Rightarrow> 'a skat" (infixl "iff" 65)
 where
-  "x iff y = !((x + y) \<cdot> !(x \<cdot> y))"
+  "x iff y = !x\<cdot>!y + x\<cdot>y"
 
 declare biconditional_def [skat_simp]
+
+lemma bicon_conj1: "\<lbrakk>x \<in> carrier tests; y \<in> carrier tests\<rbrakk> \<Longrightarrow> (x iff y)\<cdot>y = x\<cdot>y"
+  apply (simp add: biconditional_def skd.distr[simplified])
+  by (smt complement_zero de_morgan1 not_closed skd.add_comm skd.add_idem skd.add_zeror skd.mult_assoc test_double_compl)
+
+lemma bicon_conj2: "\<lbrakk>x \<in> carrier tests; y \<in> carrier tests\<rbrakk> \<Longrightarrow> y\<cdot>(x iff y) = x\<cdot>y"
+  by (smt biconditional_def complement_zero de_morgan1 de_morgan2 not_closed skd.add_zerol skd.distl skd.mult_assoc skt.test_meet_idem skt.test_mult_comm)
+
+lemma bicon_zero: "\<lbrakk>x \<in> carrier tests; y \<in> carrier tests\<rbrakk> \<Longrightarrow> (x iff y)\<cdot>(!x\<cdot>y) = \<zero>"
+  by (smt bicon_conj1 complement_zero not_closed skd.mult_assoc skd.mult_zeror skt.test_mult_comm)
+
+lemma bicon_comm: "\<lbrakk>x \<in> carrier tests; y \<in> carrier tests\<rbrakk> \<Longrightarrow> x iff y = y iff x"
+  by (metis (lifting) biconditional_def not_closed skt.test_mult_comm)
 
 definition concat_map where "concat_map f = concat \<circ> map f"
 
@@ -102,67 +179,6 @@ declare f_def [skat_simp]
 
 (* Sequences *)
 
-definition seq :: "'a::ranked_alphabet skat list \<Rightarrow> 'a skat" where
-  "seq xs = foldr op \<cdot> xs \<one>"
-
-declare seq_def [skat_simp]
-
-lemmas oner = skd.mult_oner[simplified]
-
-declare oner [skat_simp]
-
-lemma seq_singleton: "seq [v] = v"
-  by (simp add: seq_def, metis skd.mult_oner)
-
-lemma seq_mult: "seq (xs @ ys) = seq xs \<cdot> seq ys"
-  apply (induct xs)
-  apply (simp add: seq_def)
-  apply (metis skd.mult_onel)
-  apply (simp add: seq_def)
-  by (metis skd.mult_assoc)
-
-lemma list_td_split: "take n xs @ drop n xs = xs"
-  by (induct xs, simp_all)
-
-lemma seq_split:
-  assumes seq_take: "seq (take n xs) = seq (take n ys)"
-  and seq_drop: "seq (drop n xs) = seq (drop n ys)"
-  shows "seq xs = seq ys"
-proof -
-  have "seq (take n xs @ drop n xs) = seq (take n ys @ drop n ys)"
-    by (simp only: seq_mult, metis seq_drop seq_take)
-  thus ?thesis
-    by simp
-qed
-
-definition take_rev :: "nat \<Rightarrow> 'a list \<Rightarrow> 'a list" where
-  "take_rev n xs = rev (take n (rev xs))"
-
-declare take_rev_def [simp]
-
-definition drop_rev :: "nat \<Rightarrow> 'a list \<Rightarrow> 'a list" where
-  "drop_rev n xs = rev (drop n (rev xs))"
-
-declare drop_rev_def [simp]
-
-lemma take_drop_rev_id [simp]: "drop_rev n xs @ take_rev n xs = xs"
-  by (metis append_take_drop_id drop_rev_def rev_append rev_rev_ident take_rev_def)
-
-lemma seq_split_rev:
-  assumes seq_take: "seq (take_rev n xs) = seq (take_rev n ys)"
-  and seq_drop: "seq (drop_rev n xs) = seq (drop_rev n ys)"
-  shows "seq xs = seq ys"
-proof -
-  have "seq (drop_rev n xs @ take_rev n xs) = seq (drop_rev n ys @ take_rev n ys)"
-    by (simp only: seq_mult, metis seq_drop seq_take)
-  thus ?thesis
-    by (simp only: take_drop_rev_id)
-qed
-
-lemma seq_append:
-  "seq (take n xs) \<cdot> seq (drop n xs) = seq (take m ys) \<cdot> seq (drop m ys) \<Longrightarrow> seq xs = seq ys"
-  by (simp add: seq_mult[symmetric])
-
 abbreviation loop where "loop v \<equiv> skat_star (seq v)"
 
 (* Useful lemmas *)
@@ -180,6 +196,7 @@ proof -
 qed
 
 (* Denesting *)
+(*
 
 definition APPEND :: "'a list \<Rightarrow> 'a list \<Rightarrow> 'a list" where
   "APPEND \<alpha> \<beta> = \<alpha> @ \<beta>"
@@ -253,17 +270,32 @@ qed
 lemma seq_permute: "\<lbrakk>xs \<in> set (permute ys); \<And>x y. \<lbrakk>x\<in>set xs; y \<in> set ys\<rbrakk> \<Longrightarrow> x\<cdot>y = y\<cdot>x\<rbrakk> \<Longrightarrow> seq xs = seq ys"
   sorry
 
-lemma seq_zero: "last xs = !y \<Longrightarrow> seq xs \<cdot> seq(y#ys) = \<zero>"
-  sorry
+lemma seq_zero_var: "\<lbrakk>xs \<noteq> []; last xs \<cdot> y = \<zero>\<rbrakk> \<Longrightarrow> seq xs \<cdot> seq (y#ys) = \<zero>"
+  apply (subst seq_cut_rev[of _ 1])
+  apply (subgoal_tac "take_rev 1 xs = [last xs]")
+  apply (rotate_tac 2)
+  apply (erule ssubst)
+  apply (simp add: seq_singleton)
+  apply (subst seq_cons[symmetric])
+  apply (subst skd.mult_assoc[simplified])
+  apply (subst skd.mult_assoc[symmetric,simplified]) back
+  apply (erule ssubst)
+  apply (simp add: skd.mult_zeror[simplified] skd.mult_zerol[simplified])
+  apply (induct xs)
+  apply auto
+  by (smt length_greater_0_conv)
 
-lemma seq_zero_var: "last xs \<cdot> y = \<zero> \<Longrightarrow> seq xs \<cdot> seq (y#ys) = \<zero>"
-  sorry
+lemma seq_zero: "\<lbrakk>y \<in> carrier tests; xs \<noteq> []; last xs = !y\<rbrakk> \<Longrightarrow> seq xs \<cdot> seq(y#ys) = \<zero>"
+  apply (rule seq_zero_var)
+  apply auto
+  by (metis complement_zero not_closed skt.test_mult_comm)
 
 lemma seq_shunt: "(\<forall>y\<in>set xs. x\<cdot>y = y\<cdot>x) \<Longrightarrow> seq (x#xs) = seq (xs@[x])"
-  sorry
+  by (induct xs, simp, auto, metis seq_cons seq_head_comm)
 
 lemma seq_12: "seq (x#y#xs) = seq (x\<cdot>y#xs)"
-  sorry
+  by (metis seq_cons seq_def skd.mult_assoc)
+*)
 
 (* Shorthand notation *)
 
@@ -277,7 +309,7 @@ abbreviation a4 where "a4 \<equiv> a 4"
 
 declare a_def [skat_simp]
 
-lemma a_test: "a n \<in> carrier tests"
+lemma a_test [intro]: "a n \<in> carrier tests"
   by (simp add: a_def P_def, rule pred_closed)
 
 lemma a_comm: "a n \<cdot> a m = a m \<cdot> a n" by skat_comm
@@ -317,10 +349,19 @@ declare q_def [skat_simp]
 definition r :: "nat \<Rightarrow> nat \<Rightarrow> kzp skat" where
   "r i j \<equiv> i := f (f (var j))"
 
+abbreviation r13 where "r13 \<equiv> r 1 3"
+abbreviation r12 where "r12 \<equiv> r 1 2"
+
+declare r_def [skat_simp]
+
 abbreviation x1 where "x1 \<equiv> 1 := vx"
 
 definition s :: "nat \<Rightarrow> kzp skat" where
   "s i \<equiv> i := f vx"
+
+abbreviation s1 where "s1 \<equiv> s 1"
+
+declare s_def [skat_simp]
 
 definition t :: "nat \<Rightarrow> kzp skat" where
   "t i \<equiv> i := g (f vx) (f vx)"
@@ -336,7 +377,163 @@ declare z_def [skat_simp]
 abbreviation z2 where "z2 \<equiv> z 2"
 
 definition y :: "nat \<Rightarrow> kzp skat" where
-  "y i \<equiv> i := bot"
+  "y i \<equiv> i := null"
+
+declare y_def [skat_simp]
+
+ML {*
+fun NTIMES 0 _ = all_tac
+  | NTIMES n tac = tac THEN (NTIMES (n - 1) tac)
+
+fun commr_tac s c m = Subgoal.FOCUS (fn {context, ...} =>
+  let
+    val move_right_tac = EVERY
+      [ EqSubst.eqsubst_tac context [0] @{thms zip_comm} 1
+      , skat_comm_tac context 1
+      , EqSubst.eqsubst_tac context [0] @{thms zip_left} 1
+      ]
+  in
+    DETERM (zip_tac s c context 1)
+    THEN (if m = 0
+          then (CHANGED (REPEAT move_right_tac))
+          else (NTIMES m move_right_tac))
+    THEN unzip_tac context 1
+    THEN seq_deselect_tac 1
+  end)
+*}
+
+method_setup commr1 = {*
+Scan.lift Parse.nat  -- Scan.lift Parse.nat -- Scan.lift (Scan.optional Parse.nat 0) >>
+  (fn ((s, c), m) => fn ctxt => SIMPLE_METHOD' (commr_tac s c m ctxt))
+*}
+
+method_setup comml1 = {*
+Scan.lift Parse.nat  -- Scan.lift Parse.nat -- Scan.lift (Scan.optional Parse.nat 0) >>
+  (fn ((s, c), m) => fn ctxt =>
+    let
+      val move_left_tac = EVERY
+        [ EqSubst.eqsubst_tac ctxt [0] @{thms zip_comm} 1
+        , skat_comm_tac ctxt 1
+        , EqSubst.eqsubst_tac ctxt [0] @{thms zip_right} 1
+        ]
+    in
+      DETERM (zip_tac s (c - 1) ctxt 1)
+      THEN (if m = 0
+            then (CHANGED (REPEAT move_left_tac))
+            else (NTIMES m move_left_tac))
+      THEN unzip_tac ctxt 1
+      THEN seq_deselect_tac 1
+      |> SIMPLE_METHOD
+    end)
+*}
+
+ML_val {* Subgoal.FOCUS *}
+
+ML {*
+fun seq_comm_step_tac ctxt n =
+  rtac @{thm conjI} n THEN simp_tac (simpset_of ctxt) n
+  THEN rtac @{thm conjI} n THEN simp_tac (simpset_of ctxt) n
+  THEN REPEAT (rtac @{thm comms_cons} n THEN skat_comm_tac ctxt n)
+  THEN rtac @{thm comms_nil} n
+  THEN simp_tac (simpset_of ctxt) n
+
+fun destroy [] = (fn x => x)
+  | destroy (f::fs) = f o Thm.dest_comb #> destroy fs
+
+fun safe_dest_comb ctrm = SOME (Thm.dest_comb ctrm)
+  handle CTERM _ => NONE
+
+fun safe_destroy [] ctrm = SOME ctrm
+  | safe_destroy (f::fs) ctrm =
+    case (safe_dest_comb ctrm) of
+      NONE => NONE
+    | SOME x => safe_destroy fs (f x);
+
+fun ml_list ctrm =
+  case (safe_destroy [fst, snd] ctrm) of
+    NONE => []
+  | SOME x => x :: ml_list (destroy [snd] ctrm);
+
+fun find_index _ [] = 0
+  | find_index x (y::ys) =
+    (if x aconvc y then 0 else 1 + find_index x ys)
+
+fun seq_comm_get_index concl =
+  let
+    val ys = concl |> destroy [snd, snd, snd] |> ml_list
+    val xs = concl |> destroy [snd, fst, snd, snd] |> ml_list
+  in
+    find_index (hd xs) ys
+  end
+
+val seq_comm1_tac = Subgoal.FOCUS (fn {concl, context, ...} =>
+  let
+    val index = nat_cterm (seq_comm_get_index concl)
+    val exI_index = Drule.instantiate' [SOME @{ctyp "nat"}] [NONE, SOME index] @{thm exI}
+  in
+    EVERY [rtac @{thm comm_step} 1, rtac exI_index 1, seq_comm_step_tac context 1]
+    ORELSE commr_tac 1 1 0 context 1
+  end
+  handle CTERM _ => no_tac)
+
+val seq_comm_tac = Subgoal.FOCUS (fn {context, ...} =>
+  REPEAT1 (seq_comm1_tac context 1))
+*}
+
+method_setup seq_comm = {* Scan.succeed (fn ctxt => SIMPLE_METHOD' (seq_comm_tac ctxt)) *}
+
+lemma null_simp [simp]: "X ::= exp \<cdot> X ::= null = X ::= null"
+  by (metis FV_null Int_empty_right no_FV skat_set_assign3)
+
+lemma elim_inst: "halt = seq [x := null, halt]"
+  sorry
+
+lemma elim_subst: "X = Y \<Longrightarrow> X ::= x \<cdot> Y ::= null = Y ::= null"
+  sorry
+
+lemma elim_null: "qes (x := null#xs) \<cdot> seq [halt] = qes xs \<cdot> seq [halt]"
+  sorry
+
+ML {*
+fun zip_var_elim_tac ctxt n = DETERM (
+  EqSubst.eqsubst_tac ctxt [0] @{thms zip_elim_var} n
+  THEN SOLVED' (fn n =>
+    asm_full_simp_tac (simpset_of ctxt addsimps SkatSimpRules.get ctxt) n
+    THEN TRY (touch_simp_tac ctxt n)
+    THEN TRY (rtac @{thm elim_subst} n)
+    THEN TRY (simp_tac (simpset_of ctxt) n)) n)
+
+fun zip_comml_tac ctxt n = DETERM (
+  EqSubst.eqsubst_tac ctxt [0] @{thms zip_comm} n
+  THEN skat_comm_tac' skat_ni_commuter ctxt n
+  THEN EqSubst.eqsubst_tac ctxt [0] @{thms zip_right} n)
+
+fun zip_commr_tac ctxt n = DETERM (
+  EqSubst.eqsubst_tac ctxt [0] @{thms zip_comm} n
+  THEN skat_comm_tac ctxt n
+  THEN EqSubst.eqsubst_tac ctxt [0] @{thms zip_left} n)
+
+fun var_elim_tac v ctxt n =
+  let
+    val v_ctrm = nat_cterm v
+  in
+    seq_select_tac 1 ctxt n
+    THEN simp_tac (HOL_basic_ss addsimps @{thms seq_to_qes rev.simps append.simps}) n
+    THEN EqSubst.eqsubst_tac ctxt [0] @{thms qes_snoc} n
+    THEN EqSubst.eqsubst_tac ctxt [0] [Drule.instantiate' [] [SOME v_ctrm] @{thm elim_inst}] n
+    THEN REPEAT (zip_var_elim_tac ctxt n ORELSE zip_comml_tac ctxt n ORELSE manual_elim_tac)
+    THEN EqSubst.eqsubst_tac ctxt [0] @{thms zip_left} n
+    THEN REPEAT (zip_commr_tac ctxt n)
+    THEN EqSubst.eqsubst_tac ctxt [0] @{thms elim_null} n
+    THEN unzip_tac ctxt n
+    THEN seq_deselect_tac n
+  end
+*}
+
+lemma "seq [q311,q 2 3 1,q311,halt] = seq [halt]"
+  apply (tactic {* var_elim_tac 3 @{context} 1 *})
+  ML_prf {* Goal.init @{cprop "False"} *}
+  defer
 
 no_notation
   one_class.one ("1") and
@@ -407,108 +604,96 @@ declare foldr.simps[skat_simp]
 declare o_def[skat_simp]
 declare id_def[skat_simp]
 
+lemma seq_merge: "seq (Vx#Vy#Vxs) = seq (Vx\<cdot>Vy#Vxs)"
+  sorry
+
+lemma vhalt [intro]: "vy \<notin> output_vars TYPE(kzp) \<Longrightarrow> vy := vs \<cdot> halt = halt"
+  sorry
+
+lemma vhalt2 [intro]: "vy \<notin> output_vars TYPE(kzp) \<Longrightarrow> halt = vy := vs \<cdot> halt"
+  by (metis vhalt)
+
+declare output_vars_kzp_def [simp]
+
 lemma kozen1: "p41\<cdot>p11 = p41\<cdot>p11\<cdot>(a1 iff a4)"
+  sorry
+
+lemma kozen1_seq: "seq [p41,p11] = seq [p41,p11,(a1 iff a4)]"
   sorry
 
 lemma kozen2: "p41\<cdot>p11\<cdot>q214 = p41\<cdot>p11\<cdot>q211"
   sorry
 
+lemma kozen3: "p41\<cdot>p11\<cdot>q211\<cdot>q311\<cdot>a1\<cdot>a4 = p41\<cdot>p11\<cdot>q211\<cdot>q311\<cdot>a1"
+  sorry
+
+lemma kozen3_seq: "seq [p41,p11,q211,q311,a1,a4] = seq [p41,p11,q211,q311,a1]"
+  by (simp add: seq_def skd.mult_onel kozen3)
+
+lemma kozen4_seq: "seq [q211,q311,r13] = seq [q211,q311,r12]"
+  sorry
+
+lemma kozen5_seq1: "seq [q211,q311,a3] = seq [q211,q311,a2]"
+  sorry
+
+lemma kozen5_seq2: "seq [q211,q311,!a3] = seq [q211,q311,!a2]"
+  sorry
+
+lemma [simp]: "X ::= v \<cdot> X ::= null = X ::= null"
+  by (metis FV_null inf_bot_right no_FV skat_set_assign3)
+
+lemma plus_indiv: "\<lbrakk>vx1 = x2; y1 = y2\<rbrakk> \<Longrightarrow> (vx1::kzp skat) + y1 = x2 + y2"
+  by auto
+
 theorem kozen_scheme_equivalence: "seq scheme1 = seq scheme2"
 proof -
   have "seq scheme1 = seq
+    [x1,p41,p11,q214,q311,loop [!a1,p11,q214,q311],a1,p13
+    ,loop [!a4 + seq [a4,(!a2\<cdot>p22)\<^sup>\<star>,a2,!a3,p41,p11],q214,q311,loop [!a1,p11,q214,q311],a1,p13]
+    ,a4,(!a2\<cdot>p22)\<^sup>\<star>,a2,a3,z2,halt]"
+    by (simp add: scheme1_def p_def[symmetric] q_def[symmetric] a_def[symmetric] z_def[symmetric])
+
+  also have "... = seq
     [x1,p41,p11,q214,q311,loop [!a1,p11,q214,q311]
     ,loop [a1,p13,!a4 + seq [a4,(!a2\<cdot>p22)\<^sup>\<star>,a2,!a3,p41,p11],q214,q311,loop [!a1,p11,q214,q311]]
     ,a1,p13,a4,(!a2\<cdot>p22)\<^sup>\<star>,a2,a3,z2,halt]"
-    apply (simp add: scheme1_def p_def[symmetric] q_def[symmetric] a_def[symmetric] z_def[symmetric])
-    apply (rule seq_split[of 6], simp_all)
-    apply (rule seq_split[of 3], simp_all)
-    apply (rule seq_append[of 2 _ 1], simp)
-    apply (simp only: seq_singleton)
-    apply (rule HOL.trans)
-    by (rule seq_slide[of _ 4], simp_all)
+    by (cong, cut 1 2, cut 6 1, simp, cut 2 4, cut 3 2, simp only: ska.star_slide[simplified])
 
   also have "... = seq
     [x1,p41,p11,q214,q311
     ,(seq [!a1,p11,q214,q311] + seq [a1,p13,!a4 + seq [a4,(!a2\<cdot>p22)\<^sup>\<star>,a2,!a3,p41,p11],q214,q311])\<^sup>\<star>
     ,a1,p13,a4,(!a2\<cdot>p22)\<^sup>\<star>,a2,a3,z2,halt]"
-    apply (rule seq_split[of 5])
-    apply simp_all
-    apply (rule seq_split_rev[of 8])
-    apply simp_all
-    apply (subst seq_def, simp)
-    apply (subst skd.mult_oner[simplified])
-    apply (subst seq_denest_break[of _ _ 1])
-    apply simp
-    apply (simp only: APPEND_def)
-    apply (subst seq_denest)
-    by (simp only: seq_singleton)
+    by (cong, cut 1 1, cut 2 5, simp add: ska.star_denest[symmetric,simplified])
 
   also have "... = seq
     [x1,p41,p11,q214,q311
     ,(seq [!a1,p11,q214,q311] + seq [a1,p13,!a4,q214,q311] + seq [a1,p13,a4,(!a2\<cdot>p22)\<^sup>\<star>,a2,!a3,p41,p11,q214,q311])\<^sup>\<star>
     ,a1,p13,a4,(!a2\<cdot>p22)\<^sup>\<star>,a2,a3,z2,halt]"
-    apply (rule seq_split[of 5], simp_all)
-    apply (rule seq_split_rev[of 8], simp_all)
-    apply (simp add: seq_singleton)
-    apply (subst skd.add_assoc[simplified])
+    apply (cong, simp, subst skd.add_assoc[simplified])
     apply (rule_tac f = "\<lambda>x. (?v + x)\<^sup>\<star>" in arg_cong)
-    apply (simp add: seq_def skd.mult_oner)
-    apply (subst skd.distr[simplified])
-    apply (simp add: skd.mult_assoc[symmetric, simplified])
-    apply (subst skd.distl[simplified])
-    by (simp add: skd.mult_assoc[simplified])
+    apply (simp add: seq_foldr skd.mult_oner)
+    by (smt skd.distl skd.distr skd.mult_assoc)
 
   also have "... = seq
     [x1,p41,p11,q214,q311
     ,(seq [!a1,!a4,p11,q214,q311] + seq [!a1,a4,p11,q214,q311] + seq [a1,!a4,p13,q214,q311]
     + seq [a1,a4,p13,(!a2\<cdot>p22)\<^sup>\<star>,a2,!a3,p41,p11,q214,q311])\<^sup>\<star>
     ,(!a2\<cdot>p22)\<^sup>\<star>,a1,a2,a3,a4,z2,halt]"
-    apply (rule seq_split[of 5], simp_all)
-    apply (rule seq_match)
+    apply congl
+    apply (rule seq_head_eq)
     apply (rule arg_cong) back
     apply (rule plus_indiv)+
-    apply (rule seq_plus_head_r)
-    apply (subst seq_plus_elim)
-    apply (rule a_test, simp)
-    apply (rule seq_split[of 1], simp_all)
-    apply (rule seq_split_rev[of 2], simp_all)
-    apply (simp add: seq_def skd.mult_oner)
-    apply skat_comm
-    apply (rule seq_split[of 1], simp_all)
-    apply (rule seq_split_rev[of 7], simp_all)
-    apply (simp add: seq_def)
-    apply skat_comm
-    apply (subst seq_head_comm) back
-    apply skat_comm
-    apply (subst seq_split[of 1], simp_all)
-    apply (subgoal_tac "halt = p13 \<cdot> halt")
-    apply (erule ssubst) back
-    apply (subst seq_cut[of _ 1], simp_all)
-    apply (subst seq_def, simp add: skd.mult_oner[simplified])
-    apply (subst seq_empty)
-    apply (subst seq_push, skat_comm)+
-    apply (subst skd.mult_assoc[simplified])
-    apply (subst seq_snoc)
-    apply (simp add: seq_singleton)
-    apply (subst seq_split_rev[of 2], simp_all)
-    apply (subst seq_head_comm, skat_comm, subst seq_split[of 1], simp_all)+
-    apply (subst skat_halt[of 1]) back
-    apply (simp add: output_vars_kzp_def)
-    apply (simp add: p_def)
-    apply (subst skd.mult_assoc[symmetric,simplified])
-    apply (subst skat_null_zero)
-    apply (subst skat_halt[symmetric])
-    apply (simp add: output_vars_kzp_def)
-    by simp
+    apply (auto simp add: seq_head_elim_var[OF a_test])
+    apply seq_comm+
+    by (auto simp add: seq_foldr mult_oner p_def)
 
   also have "... = seq
     [x1,p41,p11,q214,q311
     ,(seq [!a1,a4,p11,q214,q311]
     + seq [a1,a4,p13,(!a2\<cdot>p22)\<^sup>\<star>,a2,!a3,p41,p11,q214,q311])\<^sup>\<star>
     ,(!a2\<cdot>p22)\<^sup>\<star>,a1,a2,a3,a4,z2,halt]"
-    apply (subst seq_split[of 5], simp_all)
-    apply (subst seq_cons[symmetric])
-    apply (subst seq_cons[symmetric]) back back back back back
+    apply congl
+    apply (cut 1 1, simp, cut 6 1, simp)
     apply (subst skd.add_assoc[simplified])
     apply (subst skd.add_comm[simplified]) back
     apply (subst skd.add_assoc[symmetric,simplified])
@@ -518,13 +703,10 @@ proof -
     apply (erule ssubst)
     apply (subgoal_tac "seq [a1,!a4,p13,q214,q311] = seq [a1,p13,q214,q311,!a4]")
     apply (erule ssubst)
-    apply (subst seq_head_comm) back back
-    apply skat_comm
-    apply (subst seq_head_comm) back back back
-    apply skat_comm
+    apply (commr 3 1)
+    apply (commr 4 1)
     apply (simp add: skd.distr[simplified] skd.distl[simplified])
-    apply (subst seq_zero, simp)+
-    apply (simp add: skd.add_zerol)
+    apply (zero, auto simp add: skd.add_zerol)+
     prefer 3
     apply (subgoal_tac "seq [(!a2\<cdot>p22)\<^sup>\<star>,a1,a2,a3,a4,z2,halt] = seq [a4,(!a2\<cdot>p22)\<^sup>\<star>,a1,a2,a3,z2,halt]")
     apply (erule ssubst)
@@ -533,77 +715,140 @@ proof -
     apply (subgoal_tac "seq [a1,!a4,p13,q214,q311] = seq [a1,p13,q214,q311,!a4]")
     apply (erule ssubst)
     apply (simp add: skd.distr[simplified])
-    apply (subst seq_zero,simp)+
-    apply (simp add: skd.add_zerol)
-    prefer 3
-    apply (subst seq_head_comm) back
-    apply skat_comm
-    apply (subst seq_split[of 1], simp_all)
-    apply (subst seq_split_rev[of 2], simp_all)
-    apply (rule seq_permute)
-    apply simp
-    apply (simp, safe)
-    apply skat_comm+
-    apply (subst seq_split[of 1], simp_all)
-    apply (subst seq_shunt, simp, safe, skat_comm+, simp)
-    apply (subst seq_split[of 1], simp_all)
-    by (subst seq_shunt, simp, safe, skat_comm+, simp)
+    apply (zero, auto simp add: skd.add_zerol)+
+    by seq_comm+
 
   also have "... = seq
     [x1,p41,p11,q214,q311
     ,(seq [a1,a4,p13,(!a2\<cdot>p22)\<^sup>\<star>,a2,!a3,p41,p11,q214,q311])\<^sup>\<star>
     ,(!a2\<cdot>p22)\<^sup>\<star>,a1,a2,a3,a4,z2,halt]"
-    apply (subst seq_split_rev[of 7], simp_all)
-    apply (subst seq_def)
-    apply (subst seq_def) back back
+    apply congr
+    apply (subst seq_foldr)
+    apply (subst seq_foldr) back back
     apply (simp add: skd.mult_assoc[symmetric,simplified] skd.mult_oner[simplified])
     apply (rule ska.kozen_skat_lemma_dual[simplified])
-    defer
+    apply (cut 1 6, cut 2 2, seq_select 2, subst kozen1_seq, seq_deselect)
+    apply (subst seq_mult[symmetric], subst seq_mult[symmetric], simp)
+    apply (commr 1 9) apply (subst seq_merge) back
+    apply (subst zippify, simp, rule zip_zero)
+    apply (metis (lifting) a_test bicon_zero)
     apply (subst skd.mult_assoc[simplified])
     apply (subst kozen1)
     apply (simp add: skd.mult_assoc[symmetric,simplified])
-    apply (subst seq_empty)
-    apply (subst seq_snoc)+
-    apply (subst seq_snoc[symmetric])
-    apply simp
-    apply (subst seq_cut[of _ 3], simp)
-    apply (subst seq_shunt) back
-    apply (simp, safe)
-    apply skat_comm+
-    apply simp
-    apply (subst seq_12) back back
-    apply (subst skd.mult_assoc[simplified])
-    apply (subst seq_zero_var)
-    apply (simp add: biconditional_def)
-    defer
-    apply (metis skd.mult_zeror)
-    apply (subst seq_cut[of _ 6], simp)
-    apply (subst seq_cut[of _ 2]) back apply simp
-    apply (subst seq_def) back
-    apply (simp add: skd.mult_oner[simplified])
-    apply (subst kozen1)
-    apply (subst skd.mult_assoc[simplified]) back
-    apply (subst seq_cons)
-    apply (simp add: skd.mult_assoc[simplified])
-    apply (subst seq_shunt) back
-    apply (simp, safe)
-    apply skat_comm+
-    apply simp
-    apply (subst seq_12) back back
-    apply (subst seq_zero_var)
-    apply simp
-    prefer 2
-    apply (simp add: skd.mult_zeror[simplified])
-    apply (simp add: biconditional_def)
-    sorry
+    apply (subst seq_singleton[symmetric])
+    apply seq_rev
+    apply (subst qes_snoc[symmetric])+
+    apply (subst qes_snoc)
+    apply qes_rev
+    apply (commr 1 4)
+    apply (subst seq_merge) back
+    apply (subst zippify, simp, rule zip_zero)
+    by (metis (lifting) a_test bicon_zero)
 
   also have "... = seq
     [x1,p41,p11,q211,q311
     ,(seq [a1,a4,p13,(!a2\<cdot>p22)\<^sup>\<star>,a2,!a3,p41,p11,q211,q311])\<^sup>\<star>
     ,(!a2\<cdot>p22)\<^sup>\<star>,a1,a2,a3,a4,z2,halt]"
-    apply (simp add: seq_def)
-    apply (simp add: skd.mult_assoc[symmetric,simplified] skd.mult_oner[simplified])
-    by (smt kozen2 skd.mult_assoc)
+    by (simp add: seq_def skd.mult_onel[simplified], smt kozen2 skd.mult_assoc)
+
+  also have "... = seq
+    [x1,(seq [p41,p11,q211,q311,a1,a4,p13,(!a2\<cdot>p22)\<^sup>\<star>,a2,!a3])\<^sup>\<star>
+    ,p41,p11,q211,q311,(!a2\<cdot>p22)\<^sup>\<star>,a1,a2,a3,a4,z2,halt]"
+    by (cong, cut 1 4, cut 3 6, cut 6 4, cut 5 1, simp add: ska.star_slide)
+
+  also have "... = seq
+    [x1,(seq [p41,p11,q211,q311,a1,p13,(!a2\<cdot>p22)\<^sup>\<star>,a2,!a3])\<^sup>\<star>
+    ,p41,p11,q211,q311,a1,(!a2\<cdot>p22)\<^sup>\<star>,a2,a3,z2,halt]"
+    apply (cut 2 6, zip 1 7, subst zip_comm, skat_comm)
+    apply (zip 3 3)
+    apply (subst zip_comm, skat_comm, subst zip_right)+
+    apply (unzip+, cut 1 2, cut 4 6)
+    apply (simp add: kozen3_seq)
+    by (subst seq_mult[symmetric], simp)+
+
+  also have "... = seq
+    [x1,(seq [p41,p11,q211,q311,a1,p13,(!a2\<cdot>p22)\<^sup>\<star>,a2,!a3])\<^sup>\<star>
+    ,p41,p11,q211,q311,(!a2\<cdot>p22)\<^sup>\<star>,a1,a2,a3,z2,halt]"
+    by (congr, zip 3 7, subst zip_comm, skat_comm, unzip, seq_deselect)
+
+  also have "... = seq
+    [x1,(seq [p11,q211,q311,a1,p13,(!a2\<cdot>p22)\<^sup>\<star>,a2,!a3])\<^sup>\<star>
+    ,p11,q211,q311,(!a2\<cdot>p22)\<^sup>\<star>,a1,a2,a3,z2,halt]"
+    apply (cut 1 11)
+    apply (subgoal_tac "halt = seq[y 4, halt]", erule ssubst) back back
+    apply (simp add: seq_singleton seq_mult[symmetric])
+    apply (zip 1 11)
+    apply (subst zip_comm, skat_comm, subst zip_right)+
+    apply (unzip, seq_deselect)
+    apply (subst seq_cons) back
+    apply (zip 1 2)
+    apply (subst seq_cons, subst qes_snoc)
+    apply (subst skd.mult_assoc[symmetric,simplified])
+    apply (subst skd.mult_assoc[simplified])
+    apply (seq_deselect)
+    apply (subst ska.star_elim[symmetric,simplified])
+    apply (metis (lifting) skat_null_zero y_def)
+    apply skat_comm+
+    apply (metis (lifting) p_def skat_null_zero y_def)
+    apply (simp add: qes_singleton skd.mult_assoc[simplified])
+    apply (subst seq_cons[symmetric])+
+    apply (zip 1 3)
+    apply (subst zip_comm, skat_comm)
+    apply (subst qes_snoc, subst seq_cons)
+    apply (subst skd.mult_assoc[simplified,symmetric])
+    apply (subst skd.mult_assoc[simplified])
+    apply (subgoal_tac "p41 \<cdot> y 4 = y 4", erule ssubst)
+    apply (subst qes_snoc[symmetric])
+    apply (subst zip_comm, skat_comm, subst zip_left)+
+    apply (unzip, seq_deselect)
+    apply (seq_rev)
+    apply (subst qes_snoc, subst qes_snoc)
+    apply (subst skd.mult_assoc[simplified])
+    apply (subgoal_tac "y 4 \<cdot> halt = halt", erule ssubst)
+    apply (subst qes_snoc[symmetric])
+    apply (simp add: qes_def)
+    apply (simp add: y_def)
+    apply (insert output_vars_kzp_def[of "TYPE(kzp)"])
+    apply (smt singletonE vhalt)
+    apply (metis (lifting) p_def skat_null_zero y_def)
+    by (smt seq_cons seq_singleton singleton_iff vhalt2 y_def)
+
+  also have "... = seq
+    [x1,p11,(seq [q211,q311,(!a2\<cdot>p22)\<^sup>\<star>,a1,a2,!a3,p13,p11])\<^sup>\<star>
+    ,q211,q311,(!a2\<cdot>p22)\<^sup>\<star>,a1,a2,a3,z2,halt]"
+    by (commr 2 5, commr1 2 4 1, simp add: seq_def mult_onel, smt ska.star_slide skd.mult_assoc)
+
+  also have "... = seq
+    [s1,(seq [q211,q311,(!a2\<cdot>p22)\<^sup>\<star>,a1,a2,!a3,r13])\<^sup>\<star>
+    ,q211,q311,(!a2\<cdot>p22)\<^sup>\<star>,a1,a2,a3,z2,halt]"
+    sorry
+
+  also have "... = seq
+    [s1,(seq [a1,q211,q311,r13,(!a2\<cdot>p22)\<^sup>\<star>,a2,!a3])\<^sup>\<star>
+    ,q211,q311,(!a2\<cdot>p22)\<^sup>\<star>,a1,a2,a3,z2,halt]"
+    by (comml 2 4, comml 2 7)
+
+  also have "... = seq
+    [s1,(seq [a1,q211,q311,!a2,r12,(!a2\<cdot>p22)\<^sup>\<star>,a2])\<^sup>\<star>
+    ,q211,q311,a2,(!a2\<cdot>p22)\<^sup>\<star>,a1,a2,z2,halt]"
+    apply (cut 2 1)
+    apply (cut 3 3)
+    apply (simp only: kozen4_seq seq_mult[symmetric] append.simps)
+    apply (comml 2 7, comml 1 8, cut 1 2, cut 3 3, cut 2 1, cut 3 3)
+    apply (simp add: kozen5_seq1 kozen5_seq2)
+    by (simp add: seq_def mult_onel skd.mult_assoc[simplified])
+
+  also have "... = seq
+    [s1,(seq [a1,q211,!a2,(!a2\<cdot>p22)\<^sup>\<star>,a2])\<^sup>\<star>
+    ,q211,a2,(!a2\<cdot>p22)\<^sup>\<star>,a1,a2,z2,halt]"
+    apply (tactic {* var_elim_tac 3 @{context} 1 *})
+    apply (subgoal_tac "halt = y 3 \<cdot> halt", erule ssubst) back back
+    apply (seq_rev, subst qes_snoc)
+    apply (subst skd.mult_assoc[symmetric,simplified])
+    apply (subst qes_snoc[symmetric])+
+    apply (qes_rev)
+    apply (comml1 1 10 5)
+    apply (zip 1 4)
     
 
   also have "... = seq scheme2"
